examples

trunk/examples/programs/toy/tooDifficultLoopInvariant/GasCakeWithJohoFractions01HardcodedInput.bpl
@@ -5,7 +5,7 @@
  */
 
 procedure main() returns () {
-    var input : real;
+//     var input : real;
     var output : real;
 	var internal : real;
 	internal := 0.0;
@@ -13,11 +13,10 @@ procedure main() returns () {
 	while (true) 
 // 	invariant (internal * (9.0 / 10.0) + output >= 0.0 && internal * (9.0 / 10.0) + output <= 100.0);
 	{
- 		havoc input;
- 		input := 100.0;
+// 		havoc input;
+// 		input := 100.0;
 // 		assume (input >= 0.0 && input <= 100.0);
 		output, internal := output + internal * 0.02, 100.0 * (2.0 / 81.0) + (output * (2.0 / 81.0) * -1.0 + internal * (43.0 / 45.0));
-		assert 0.0 <= output; 
-		assert output <= 100.0;
+		assert 0.0 <= output && output <= 100.0;
 	}
 }
