trunk/examples/programs/toy/tooDifficultLoopInvariant/GasCakeWithJohoFractions01.bpl
@@ -14,8 +14,8 @@ procedure main() returns () {
 // 	invariant (internal * (9.0 / 10.0) + output >= 0.0 && internal * (9.0 / 10.0) + output <= 100.0);
 	{
  		havoc input;
- 		input := 100.0;
-// 		assume (input >= 0.0 && input <= 100.0);
+//  		input := 100.0;
+		assume (input >= 0.0 && input <= 100.0);
 		output, internal := output + internal * 0.02, 100.0 * (2.0 / 81.0) + (output * (2.0 / 81.0) * -1.0 + internal * (43.0 / 45.0));
 		assert 0.0 <= output; 
 		assert output <= 100.0;
